linarith/and_of_map.lean
@@ -1,0 +1,99 @@
+/-
+Copyright (c) 2017 Robert Y. Lewis. All rights reserved.
+Released under Apache 2.0 license as described in the file LICENSE.
+Author: Robert Y. Lewis
+-/
+
+import ..algebra.order ..data.fin
+open nat tactic
+
+def and_of_map_aux (n : ℕ) (f : fin n → Prop) : Π k, k < n → Prop
+| 0 h := f (fin.mk 0 h)
+| (k + 1) h := (and_of_map_aux k (lt_of_succ_lt h)) ∧ f (fin.mk (k+1) h)
+
+def and_of_map : Π {n : ℕ}, (fin n → Prop) → Prop
+| 0 P := true
+| (k+1) P := and_of_map_aux (k+1) P k (lt_succ_self _)
+
+
+theorem and_of_map_aux_of_forall (n : ℕ) (P : fin n → Prop) (H : ∀ n : fin n, P n) : Π k, Π p : k < n, and_of_map_aux n P k p
+| 0 p := H _
+| (k+1) p := and.intro (by apply and_of_map_aux_of_forall) (H _)
+
+theorem and_of_map_of_forall : Π {n : ℕ} {P : fin n → Prop} (H : ∀ k : fin n, P k), and_of_map P
+| 0 P H := trivial
+| (k+1) P H := and_of_map_aux_of_forall _ _ H _ _
+
+lemma eq_of_ge_of_lt_succ {n k : ℕ} (h1 : k ≥ n) (h2 : k < n+1) : k = n := 
+have n = k ∨ n < k, from nat.eq_or_lt_of_le h1,
+or.elim this
+ (suppose n = k, eq.symm this)
+ (suppose n < k, have n+1 < n+1, from calc
+   n+1 ≤ k   : succ_le_of_lt this
+   ... < n+1 : h2,
+  absurd this (lt_irrefl _))
+
+lemma eq_zero_of_lt_one {n : ℕ} (Hn : n < 1) : n = 0 := 
+eq_zero_of_le_zero (le_of_lt_succ Hn)
+
+def fin_lower {n : ℕ} (v : fin (succ n)) (h : v^.val < n) : fin n := ⟨v^.val, h⟩
+
+def fin_prop_lower {n : ℕ} (P : fin (succ n) → Prop) : fin n → Prop := λ v, P ⟨v^.val, lt_succ_of_lt v^.is_lt⟩
+
+theorem of_fin_prop_lower (n : ℕ) (P : fin (succ n) → Prop) (v : fin (succ n)) (h : v^.val < n) 
+        (hvp : fin_prop_lower P (fin_lower v h)) : P v := 
+begin
+ unfold fin_prop_lower at hvp, unfold fin_lower at hvp,
+ dsimp at hvp,
+ assert h' : v = {val := v^.val, is_lt := v^.is_lt}, 
+ induction v,
+ apply congr,
+ reflexivity,
+ reflexivity,
+ rw h',
+ apply hvp
+end
+
+theorem and_of_map_aux_lower {n : ℕ} {P : fin (succ n) → Prop}  (k) (h : k < n) 
+        (h2 : and_of_map_aux (n+1) P k (lt_succ_of_lt h)) :
+        and_of_map_aux n (fin_prop_lower P) k h := 
+begin
+ induction k,
+ apply h2,
+ unfold and_of_map_aux,
+ split,
+ apply ih_1,
+ apply and.left h2,
+ apply and.right h2
+end
+
+theorem and_of_map_lower {n : ℕ} {P : fin (succ n) → Prop} (H : and_of_map P) : and_of_map (fin_prop_lower P) := 
+begin
+ induction n,
+ triv,
+ apply and_of_map_aux_lower,
+ apply and.left H
+end
+
+theorem forall_of_and_of_map : Π {n : ℕ} {P : fin n → Prop} (H : and_of_map P) (k : fin n), P k
+| 0 P H (fin.mk val is_lt) := absurd is_lt (not_lt_zero _)
+| 1 P H (fin.mk val is_lt) := 
+  have H1 : val = 0, from eq_zero_of_lt_one is_lt, 
+  begin revert is_lt, rw H1, intro, apply H  end
+| (n+2) P H k :=
+  begin 
+   induction k, 
+   cases (decidable.em (val < n+1)), 
+   {apply @of_fin_prop_lower _ _ (fin.mk val is_lt) a,
+   apply forall_of_and_of_map,
+   apply and_of_map_lower,
+   apply H},
+   {assert veq : val = n+1,
+   apply eq_of_ge_of_lt_succ,
+   apply le_of_not_gt a,
+   apply is_lt,
+   revert is_lt,
+   rw veq,
+   intro,
+   apply and.right H}
+  end
